add example

MLIR/Dialects/ScfSemantics.lean
@@ -83,14 +83,9 @@ def INPUT: SSAEnv arith := SSAEnv.One [⟨"x", MLIRType.i1, 0⟩]
 
   
 
-set_option pp.analyze true in 
-theorem scf_if_sem:
-  denoteBBStmt (Δ := scf)
-     (BasicBlockStmt.StmtOp
-     (Op.mk "scf.if" [SSAVal.SSAVal "b"] [] [r1, r2] (AttrDict.mk [])
-     (MLIRType.fn (MLIRType.tuple [MLIRType.int Signedness.Signless 1])
-                  (MLIRType.tuple [])))) =
-(Fitree.Vis
+def rhs (r1 r2: Region scf):
+  Fitree (UBE +' SSAEnvE scf +' Semantics.E scf) (BlockResult scf) :=
+  (Fitree.Vis
     (Sum.inr
       (Sum.inl
         (SSAEnvE.Get (ε := fun x => Unit) (MLIRType.int (ε := fun x => Unit) Signedness.Signless 1)
@@ -107,14 +102,24 @@ theorem scf_if_sem:
           Fitree (UBE +' SSAEnvE (ε := fun x => Unit) scf +' Semantics.E (ε := fun x => Unit) scf) x))
       (if (r == 0) = true then Fitree.Vis (Sum.inl (RegionE.RunRegion (ε := fun x => Unit) 0 [])) Fitree.ret
       else Fitree.Vis (Sum.inl (RegionE.RunRegion (ε := fun x => Unit) 1 [])) Fitree.ret :
-        Fitree (RegionE (ε := fun x => Unit) scf +' UBE +' ScfE) (BlockResult (ε := fun x => Unit) scf)) :
-    Fitree (UBE +' SSAEnvE (ε := fun x => Unit) scf +' Semantics.E (ε := fun x => Unit) scf)
-      (BlockResult (ε := fun x => Unit) scf))
+        Fitree (RegionE (ε := fun x => Unit) scf +' UBE +' ScfE) (BlockResult (ε := fun x => Unit) scf)))
+
+set_option pp.analyze true in 
+theorem scf_if_sem:
+  (denoteBBStmt (Δ := scf)
+     (BasicBlockStmt.StmtOp
+     (Op.mk "scf.if" [SSAVal.SSAVal "b"] [] [r1, r2] (AttrDict.mk [])
+     (MLIRType.fn (MLIRType.tuple [MLIRType.int Signedness.Signless 1])
+                  (MLIRType.tuple []))))) = rhs r1 r2
 := by {
   simp [denoteBBStmt, denoteOp, Semantics.semantics_op]
   simp_itree
   simp [scf_semantics_op];
   simp_itree;
+  -- copy state from here and paste into rhs
+  unfold rhs;
+  rfl;
+  -- tactic 'rfl' failed...
 }
 
 /-
